

Homework 4 Solutions

Ch 12: 1, 2, 9, 22 - 26, 60, 63

1. 2×2 matrices over \mathbb{Z}_2 is finite and non-commutative. Since

$$\begin{bmatrix} 1 & 1 \\ 0 & 1 \end{bmatrix} \begin{bmatrix} 1 & 1 \\ 1 & 0 \end{bmatrix} = \begin{bmatrix} 0 & 1 \\ 1 & 0 \end{bmatrix} \text{ while } \begin{bmatrix} 1 & 1 \\ 1 & 0 \end{bmatrix} \begin{bmatrix} 1 & 1 \\ 0 & 1 \end{bmatrix} = \begin{bmatrix} 1 & 0 \\ 1 & 1 \end{bmatrix}$$

2×2 matrices with entries from $2\mathbb{Z}$ would be an example of infinite, non-commutative with no unit.

2. Consider $R = 2\mathbb{Z}_{10} = \{0, 2, 4, 6, 8\}$. 6 is unity since $(5+1)(2m) = 10m + 2m = 2m \pmod{10}$ (or by inspection if you prefer). To see that each element is a unit, check $2 \cdot 8 = 6 \pmod{10}$, $4 \cdot 4 = 6 \pmod{10}$.

9. This is sort of a standard type of result you should expect. If $R = \bigcap R_i$ then we need to show closure under operations, but this is trivial since each R_i is closed.

22. Let $u, v \in U(R)$, then $(u \cdot v) \cdot (v^{-1} \cdot u^{-1}) = (u(vv^{-1})u^{-1}) = u1u^{-1} = uu^{-1} = 1$, so $v^{-1}u^{-1} = (uv)^{-1}$ and thus uv is a unit if u and v are such. The rest is even simpler.

23. Determine $U(\mathbb{Z}[i])$ we need $(a+bi)(c+di) = 1$ so $(ac-bd) = 1$ while $(ad+bc) = 0$. The only units are ± 1 and $\pm i$ are units. That these are the only units can be seen thus

$$(a+bi)^{-1} = \frac{a-bi}{a^2+b^2}$$

so $a+bi \in \mathbb{Z}[i]$ iff $\frac{a}{a^2+b^2}, \frac{b}{a^2+b^2} \in \mathbb{Z}$, for this we must have $a = \pm 1$ and $b = 0$ or $b = \pm 1$ and $a = 0$.

24. Show that $U(R_1 \times R_2 \times \cdots \times R_n) = U(R_1) \times U(R_2) \times \cdots \times U(R_n)$.

It would suffice to consider $n = 2$ and use induction. Suppose $(r, s) \in U(R_1 \times R_2)$ so there is (r', s') such that $(r, s)(r', s') = (1, 1)$, but then $(r, s) \in U(R_1) \times U(R_2)$. Essentially the same argument works in the other direction.

25. Determine $U(\mathbb{Z}[x])$. Let $p = a + p_1(x)x$ and $q = b + q_1(x)x$ then $pq = (ab + (aq_1(x) + bp_1(x))x + p_1(x)q_1(x)x^2 = 1$ iff $(a, b) = \pm(1, 1)$. So $U(\mathbb{Z}[x]) = U(\mathbb{Z})$.

26. Determine $U(\mathbb{R}[x])$. This is like the above, the only $f \in \mathbb{R}[x]$ with a multiplicative inverse is $f = a \in \mathbb{R}^* = U(\mathbb{R})$. So $U(\mathbb{R}[x]) = U(\mathbb{R})$.

60. Show that $4x^2 + 6x + 3$ is a unit in $\mathbb{Z}_8[x]$.

Here is a fun way to attack this one: Use long division! Divide 1 by $4x^2 + 6x + 3$. The trick is to note that $1 = 8x^3 + 8x^2 + 8x + 1$, then

$$\begin{array}{r}
2x+3 \\
4x^2+6x+3 \overline{) 8x^3+8x^2+8x+1} \\
\underline{8x^3+12x^2+6x} \\
-4x^2+2x+1 \\
\underline{12x^2+18x+9} \\
-8x^2-16x-8=0
\end{array}$$

Why 3 and not -1?

So $(4x^2+6x+3)(2x+3) = 8x^3+8x^2+8x+1 = 1$ and we have $(4x^2+6x+3)^{-1} = 2x+3$.

63. $A \in M_2(\mathbb{Z})$ We know $\det(AB) = \det(A)\det(B)$ and so if $AB = I$, then $\det(A)\det(B) = 1$ and as $\det(A), \det(B) \in \mathbb{Z}$ it must be that $\det(A) = \pm 1$.

Ch 13: 7, 12, 17, 30, 43, 49, 51, 56, 57, 64

7. Let R be a finite commutative ring with unity. Show that every $r \in R$ is either a unit or a 0-divisor.

Suppose r is not a zero-divisor. Consider the map $s \mapsto rs$. If $rs = rs'$, then $rs - rs' = r(s - s') = 0$. If $s \neq s'$ for any $s, s' \in R$, then r is a 0-divisor. Else, the map is 1-1 and hence onto, so $rs = 1$ for some s . (**A counting argument.**)

Any time you have an integral domain that is not a field you have non-zero-divisor non-unit elements, like 2 in \mathbb{Z} .

Note This shows that every finite integral domain is a field!

12. In \mathbb{Z}_7 give interpretations for $1/2$, $-2/3$, $\sqrt{-3}$, and $-1/6$.

$2 \cdot 4 = 1 \pmod{7}$ so $4 = 1/2 \pmod{7}$.

$1/3 = 5 \pmod{7}$ since $3 \cdot 5 = 15 = 1 \pmod{7}$ and so $2/3 = 10 = 3 \pmod{7}$ and this makes sense as $3 \cdot 3 = 9 = 2 \pmod{7}$ and so $-2/3 = -3 = 4 \pmod{7}$.

$-3 = 4 \pmod{7}$ so $2 = \sqrt{-3} \pmod{7}$, that is, $2^2 = 4 = -3 \pmod{7}$. What about $-2 = 5 \pmod{7}$? $(-2)^2 = 5^2 = 25 = 4 \pmod{7}$, do yes, 2 and -2 both satisfy $x^2 = -3$.

$1/6 = 6$ since $6 \cdot 6 = 1 \pmod{7}$ and so $-1/6 = -6 = 1 \pmod{7}$.

All pretty strange:)

17. In an integral domain if $a_1 a_2 \cdots a_n = 0$, then for some i , $a_i = 0$. So if $r^n = 0$, then $r = 0$.

30. $\mathbb{Q}[\sqrt{d}]$ is a field for d an integer. Closure under addition and multiplication are obvious and

$$a + b\sqrt{d} \cdot \frac{a - b\sqrt{d}}{a^2 - b^2 \cdot d} = 1$$

so

$$(a + b\sqrt{d})^{-1} = \frac{a}{a^2 - b^2 \cdot d} - \frac{b}{a^2 - b^2 \cdot d} \sqrt{d}$$

43. Show that $\mathbb{Z}_7[\sqrt{3}]$ is a field. The additive group part is clear essentially being isomorphic to $\mathbb{Z}_7 \times \mathbb{Z}_7$.

The multiplication is $(a + b\sqrt{3})(c + d\sqrt{3}) = (ac + 3bd) + (ad + bc)\sqrt{3}$. This will satisfy all the rules except possibly having inverses, so consider

$$1 = (a + b\sqrt{3}) \left(\frac{a - b\sqrt{3}}{(a + b\sqrt{3})(a - b\sqrt{3})} \right)$$

This will be true if $\mathbb{Z}_7[\sqrt{3}]$ is a field. So the proposed inverse of $a + b\sqrt{3}$ is

$$\left(\frac{a}{a^2 - 3b^2} \right) - \left(\frac{b}{a^2 - 3b^2} \right) \sqrt{3}$$

For this to work we need that $a^2 - 3b^2 \neq 0$ in \mathbb{Z}_7 when a and b are not both 0.

Suppose $a^2 = 3b^2 \pmod{7}$. In this case we would have $3 = (a/b)^2$, so we can't have $a^2 = 3b^2$ unless 3 is a square in \mathbb{Z}_7 .

We can just check that $m^2 \pmod{7} \neq 3$ for $m = 0, 1, \dots, 6$.

This indicates what is needed in general, $\mathbb{Z}_p[\sqrt{k}]$ is a field provided that k is not a square in \mathbb{Z}_p .

49. Let x_1, \dots, x_n belong to a ring with prime characteristic p . First notice $(x + y)^p = x^p + \binom{p}{1}x^{p-1}y + \binom{p}{2}x^{p-2}y^2 + \dots + \binom{p}{p-1}xy^{p-1} + y^p$. All of the middle terms have a factor of p and hence become 0. Thus $(x + y)^p = x^p + y^p$. Now then $(x + y)^{p^2} = ((x + y)^p)^p = (x^p + y^p)^p = (x^p)^p + (y^p)^p = x^{p^2} + y^{p^2}$, etc. By induction on m , $(x + y)^{p^m} = x^{p^m} + y^{p^m}$.

Now $((x_1 + x_2) + x_3)^{p^m} = (x_1 + x_2)^{p^m} + x_3^{p^m} = x_1^{p^m} + x_2^{p^m} + x_3^{p^m}$. So by induction on k ,

$$(x_1 + \dots + x_k)^{p^m} = x_1^{p^m} + \dots + x_k^{p^m}$$

Questions Where did we use p is prime? Where did we use commutativity?

This shows we need the "prime" assumption: In \mathbb{Z}_4 we have $(1 + 1)^4 = 2^4 = 0 \neq (1^4 + 1^4) = 2$.

What about the commutativity issue? Consider $M_2(\mathbb{Z}_2)$. Let $x = \begin{bmatrix} 1 & 1 \\ 1 & 0 \end{bmatrix}$ and $y = \begin{bmatrix} 1 & 0 \\ 1 & 1 \end{bmatrix}$, then

$$\begin{aligned} x^2 &= \begin{bmatrix} 1 & 1 \\ 1 & 0 \end{bmatrix} \begin{bmatrix} 1 & 1 \\ 1 & 0 \end{bmatrix} = \begin{bmatrix} 0 & 1 \\ 0 & 1 \end{bmatrix} = I \\ y^2 &= \begin{bmatrix} 1 & 0 \\ 1 & 1 \end{bmatrix} \begin{bmatrix} 1 & 0 \\ 1 & 1 \end{bmatrix} = \begin{bmatrix} 1 & 0 \\ 0 & 1 \end{bmatrix} \\ x^2 + y^2 &= I + I = O \\ x + y &= \begin{bmatrix} 0 & 1 \\ 1 & 0 \end{bmatrix} \\ (x + y)^2 &= \begin{bmatrix} 0 & 1 \\ 1 & 0 \end{bmatrix} \begin{bmatrix} 0 & 1 \\ 1 & 0 \end{bmatrix} = \begin{bmatrix} 1 & 0 \\ 0 & 1 \end{bmatrix} = I \end{aligned}$$

So $x^2 + y^2 \neq (x + y)^2$.

51. Let F be a finite field of character p (we know p is a prime). What we need to see is the $|F| = p^m$ for some m . Suppose $q \mid |F|$ for some $q \neq p$, then there is a $g \in F$ with $|g| = q$, that is $qg = g + g + \dots + g = 0$, but then $g \cdot (q \cdot 1) = 0$ and so $q \cdot 1 = 0$, but then $p \mid q$. So $|F| = p^m$ for some m .

56. Find all solutions to $x^2 - x + 2$ over $\mathbb{Z}_3[i]$.

We do have $x^2 - x + 2 = x^2 + 2x - 1 = (x + 1)^2 - 2 = (x + 1)^2 + 1$ so $x = 1 \pm i$. So $x = -1 - i = 2 + 2i$ and $x = -1 + i = 2 + i$ are the two roots.

57. Consider $x^2 - 5x + 6 = (x - 2)(x - 3) = 0$ Find all solutions in \mathbb{Z}_7 , \mathbb{Z}_8 , \mathbb{Z}_{12} , and \mathbb{Z}_{14} .

\mathbb{Z}_7 is a field so $x = 2$ and $x = 3 \pmod 7$ is the only solution.

In \mathbb{Z}_8 , notice that $(x - 2)(x - 3) = (x + 6)(x + 5)$ so we have

x	0	1	2	3	4	5	6	7
$x^2 - 5x + 6$	$6 \cdot 5 = 6$	$7 \cdot 6 = 2$	$0 \cdot 7 = 0$	$1 \cdot 0 = 0$	$2 \cdot 1 = 2$	$3 \cdot 2 = 6$	$4 \cdot 3 = 4$	$5 \cdot 4 = 4$

So in \mathbb{Z}_8 we have 2, 3 as roots.

Note that $x^2 - 1 = (x - 1)(x + 1)$ has roots 1 and $-1 = 7 \pmod 8$ as indicated in the factorization, but also 3 and 5. So in \mathbb{Z}_{p^k} an n^{th} -degree polynomial may have more than n roots.

$\mathbb{Z}_{12} \simeq \mathbb{Z}_4 \times \mathbb{Z}_3$ so we can solve these separately. In \mathbb{Z}_3 we have $x^2 - 5x + 6 = x^2 + x = (x)(x + 1) = (x)(x - 2)$ in \mathbb{Z}_3 so $x = 0$ and $x = 2$ in \mathbb{Z}_3 . In \mathbb{Z}_4 we have $x^2 - 5x + 6 = x^2 + 3x + 2 = (x + 2)(x + 1)$ so $x = -2, x = -1$, that is $x = 2$ and $x = 3$. Thus the solutions are $(2, 0), (2, 2), (3, 0), (3, 2)$, these correspond to 6, 2, 3, 11 in \mathbb{Z}_{12} .

$\mathbb{Z}_{14} \simeq \mathbb{Z}_2 \times \mathbb{Z}_7$ and in \mathbb{Z}_2 $x^2 - 5x + 6 = x^2 + x = (x)(x + 1) = (x)(x - 1)$ so we have 0, 1 for roots and in \mathbb{Z}_7 we have 2 and 3 so we have $(0, 2), (0, 3), (1, 2)$, and $(1, 3)$ which corresponds to 2, 3, 9, 10.

64. In a finite field F with $|F| = n$, $|F^*| = n - 1$ and $x^{|F^*|} = 1$ for all $x \in F^*$. (Since in any group G , $g^{|G|} = e$.)

Ch 14: 10, 22, 42, 48, 51, 55, 60, 62, 67, 73, 78, 80

10. In $\mathbb{Z}[x]$ show that $(2x, 3) = (x, 3)$. Clearly, $2x \in (x, 3)$ so $(2x, 3) \subseteq (x, 3)$. Conversely, $3x \in (2x, 3)$ so $x = 3x - 2x \in (2x, 3)$.

22. Let R be a finite commutative ring and I be prime. Then R/I is a finite integral domain and hence a field. We have shown before that any finite integral domain is a field, the reason is simple, let a be a non-zero element of a finite integral domain, then $ab = ac \iff a(b - c) = 0 \iff b - c = 0 \iff b = c$, so the map $c \mapsto ac$ is 1-1 and hence onto. So $ac = 1$ for some c .

42. Show that $\mathbb{R}[x]/(x^2 + 1)$ is a field. Consider $\phi : \mathbb{R}[x] \rightarrow \mathbb{C}$ given by $x \mapsto i$ (or $x \mapsto -i$) and extended uniquely to $\mathbb{R}[x]$. Clearly, ϕ is a homomorphism and $p(x) \in \ker(\phi) \iff p(i) = 0 \iff (x - i) \mid p(x)$. Since $p(x) \in \mathbb{R}[x]$ $-i$ must also be a root, namely, z is a root of $p(x)$ iff \bar{z} is a root of $\bar{p}(z)$, so $(x - i)(x + i) = x^2 + 1 \mid p(x)$. So $(x^2 + 1) = \ker(\phi)$.

48. Let $I = \{a + bi \mid a, b \in 2\mathbb{Z}\} = 2\mathbb{Z}[i] = (2)$. So I is clearly an ideal. There will be four classes, $I, 1 + I, i + I, (1 + i) + I$ and $\mathbb{Z}[i]/I$ will be isomorphic to $\mathbb{Z}_2 \times \mathbb{Z}_2$. This is not an integral domain, since $(1 + i)(1 + i) = (1 - 1) + 2i \in 2\mathbb{Z}[i]$.

51. In $\mathbb{Z}[x]$ show that $I = \{f(x) \mid f(0) \text{ is even} \} = (x, 2)$. It is clear that $f(x) \in I \iff f(x) = p(x) \cdot x + a$ for $a \in 2\mathbb{Z}$. This has just two elements, I and $1 + I$, and $\mathbb{Z}[x]/I$ is isomorphic to \mathbb{Z}_2 . This is a field, so I is maximal, hence prime.

55. In $\mathbb{Z}_5[x]$ let $I = (x^2 + x + 2)$ find a multiplicative inverse to $(2x + 3) + I$. We are looking for $p(x)$ so that $(2x + 3)p(x) = r(x)(x^2 + x + 2) + 1$. We can do as in Ch 12.60. Use division in $\mathbb{Z}_5[x]/\langle x^2 + x + 2 \rangle$. Note that $1 = 1 + \langle x^2 + x + 2 \rangle$ so try

$$\begin{array}{r} 3x + 1 \\ 2x + 3 \overline{) x^2 + x + 3} \\ \underline{x^2 + 4x} \\ 2x + 3 \\ \underline{2x + 3} \\ 0 \end{array} \quad \begin{array}{l} (3)(2) \equiv 1 \pmod{5} \text{ and } 9 \equiv 4 \pmod{5} \\ -3 \equiv 2 \pmod{5} \end{array}$$

60. In a principal ideal domain, show that every prime ideal is maximal. Let (p) be prime, if (p) were not maximal, then, there is J so that $(p) \subset J \subset R$. But $J = (q)$ since we are in a principal ideal domain and hence $q \mid p$, and so $p = q \cdot r$. But then $p \mid q$ or $p \mid r$. Suppose $p \mid r$, then $r = p \cdot d$ and we have $p = q \cdot r = q \cdot p \cdot d$ so $p \cdot (1 - q \cdot d) = 0$ and thus $q \cdot d = 1$ and so q is a unit. This is a contradiction since $(q) \neq R$. A similar argument works if $p \mid q$. In this case, we get r as a unit, so that $(p) = (q)$, again a contradiction.

62. Showing that $N(A)$ is an ideal is straightforward. Suppose $r, s \in N(A)$ so that $r^n, s^m \in A$; let $k = \max\{m, n\}$, then $(r + s)^k = \sum_{i=0}^k \binom{k}{i} r^i s^{k-i}$. In every term either r^i or s^{k-i} will be in A since $i \geq n$ or $k - i \geq m$ for all i . So $(r + s)^k \in A$. That $r \cdot s \in N(A)$ for all $r \in R$ and $s \in N(A)$ is simpler.

Here is even more!

$$N(A) = \bigcap \{J \supset A \mid J \text{ is prime}\}$$

First notice that for any $r \in R$ with $r^n \in A$, if $A \subset J$ and J is prime, then $r^n \in J$ and hence $r \in J$ (as J is prime). So we have containment $N(A) \subseteq \bigcap \{J \supset A \mid J \text{ is prime}\}$.

Now suppose $r \notin N(A)$, then we want to find a prime ideal J with $A \subset J$ and $r \notin J$. Look at \mathcal{I} being the set of all ideals of R such that $r^n \notin I$ for any n . We can find a maximal such ideal J , we just need to show that J is prime. Suppose $a \cdot b \in J$ and $a, b \notin J$. By maximality, this means that $r^n \in (a) + J$ and $r^m \in (b) + J$ so $r^n = at + s$ and $r^m = bt' + s'$ for $t, t' \in R$ and $s, s' \in J$. This means $r^{n+m} = abtt' + ats' + bt's + ss' \in J$ which is a contradiction, so $a \in J$ or $b \in J$.

67. First notice that by the polynomial division algorithm $p(x) = ax + b \pmod{x^2 + x + 1}$ for all $p(x) \in \mathbb{Z}_2[x]$. So the elements of the field are $0, 1, x$, and $1 + x$ here $x(1 + x) + (x^2 + x + 1) = 1 + (x^2 + x + 1)$ so $x^{-1} = 1 + x$ and we see that $\mathbb{Z}_2[x]$ is a field.

73. Show that if R is a PID, then R/I is a PID for all ideals $I \subset R$. Let $J \subset R/I$ be an ideal, then $J = J'/I$ for $J' = \{r \in R \mid r + I \in J\}$. We know $J' = (p)$ in R and so $J = (p)/I = (p/I)$. So R/I is a PID.

78. Show that the characteristic of $R = \mathbb{Z}[i]/(a + bi)\mathbb{Z}[i]$ divides $a^2 + b^2$.

In [this note](#) there is a lot of information about the Gaussian integers, but here is a simple response to this question:

In any ring R with unity, if we have $n_R = 0_R$, then $\text{char}(R) \mid n$. So to show that $\text{char}(R) \mid a^2 + b^2$ we need only notice that in $\mathbb{Z}[i]/(a + bi)\mathbb{Z}[i]$, $(a^2 + b^2) + (a + bi)\mathbb{Z}[i] = 0 + (a + bi)\mathbb{Z}[i]$, or equivalently, that $a^2 + b^2 \in (a + bi)\mathbb{Z}[i]$, but $a^2 + b^2 = (a + bi)(a - bi) \in (a + bi)\mathbb{Z}[i]$.

80. Let $R = \mathbb{Z}[\sqrt{-5}]$ and $I = \{a + b\sqrt{-5} \mid a - b \text{ is even}\}$. Show that I is maximal.

Consider the map

$$\phi(a + b\sqrt{-5}) = \begin{cases} 1 & a - b \text{ is odd} \\ 0 & a - b \text{ is even} \end{cases}$$

Check that $\phi : \mathbb{Z}[\sqrt{-5}] \rightarrow \mathbb{Z}_2$ is a surjective homomorphism. The main thing is multiplication where we have

$$\phi((a + b\sqrt{-5})(c + d\sqrt{-5})) = \begin{cases} 1 & (ac - 5bd) - (ad + bc) \text{ is odd} \\ 0 & (ac - 5bd) - (ad + bc) \text{ is even} \end{cases}$$

We have

$$(ac - 5bd) - (ad + bc) = (ac + bd) - (ad + bc) - 6bd = a(c - d) + b(d - c) - 6bd = (a - b)(c - d) - 6bd$$

So $(ac - 5bd) - (ad + bc)$ is odd only when $(a - b)$ and $(c - d)$ are odd. This is what we need here.

Since \mathbb{Z}_2 is a field, I is maximal.

Ch 15: 12, 14, 26, 31, 34, 38, 40, 44, 46, 50, 65, 67

12. The point here is that if $\phi : m\mathbb{Z} \rightarrow n\mathbb{Z}$, then

$$\phi(s) = \underbrace{\phi(m) + \cdots + \phi(m)}_{s \text{ times}} = s\phi(m)$$

so clearly everything is determined by $\phi(1)$. Suppose $\phi(1) = tn$. To be onto, there is s so that $\phi(s) = stn = n$, so $st = 1$, thus $t = \pm 1$ and so $\phi(m) = \pm n$. But then we have

$$\phi(m \cdot (mn)) = mn\phi(m) = mn^2 \neq n(n^2) = n\phi(m^2) = \phi(m^2n)$$

So the map cannot work unless $n = m$, in which case, $\phi(m) = m$, identity map, and $\phi(m) = -m$, negative map are the two isomorphisms.

Note: The following argument does not work. Since $\mathbb{Z}/m\mathbb{Z} = \mathbb{Z}_m \not\cong \mathbb{Z}_n = \mathbb{Z}/n\mathbb{Z}$, $m\mathbb{Z} \not\cong n\mathbb{Z}$. For this, we would require that

$$I \simeq J \implies R/I \simeq R/J$$

which is not true, for example, in $R = \mathbb{Z}[x_1, x_2, \dots]$ we have $I = \langle x_1, x_2, \dots \rangle$ and $J = \langle x_2, x_3, \dots \rangle$ so that $I \simeq J$ by the map $x_i \mapsto x_{i+1}$. But $R/I \simeq \mathbb{Z}$ while $R/J \simeq \mathbb{Z}[x]$.

It is true in this example that neither of R/I or R/J is finite, so perhaps this short argument might be saved, but I do not see it.

14. Show that $\mathbb{Z}_3[i] \simeq \mathbb{Z}_3[x]/(x^2 + 1)$. Nothing is special about 3 here except that it is prime, so \mathbb{Z}_3 is a field.

Define $\phi : \mathbb{Z}_3[x] \rightarrow \mathbb{Z}_3[i]$ by $\phi(f(x)) = f(i)$, this is clearly a ring homomorphism. (This sort of evaluation map is always a homomorphism.) The map is clearly onto as $\phi(a + bx) = a + bi$. $f(x) \in \ker(\phi)$ iff $f(i) = 0$. Since the coefficients are in \mathbb{Z}_3 we have $\overline{f(i)} = \overline{f(-i)} = f(-i) = 0$. this by the division algorithm we have that $(x - i)(x + i) = x^2 + 1 \mid f(x)$ since if not $f(x) = (x^2 + 1)q(x) + (ax + b)$ so $f(i) = b + ia = 0$ and so $a = b = 0$.

26. Determine all ring homomorphisms $\phi : \mathbb{Z}_n \rightarrow \mathbb{Z}_n$.

If we insist that $\phi(1) = 1$, i.e., that ϕ is a homomorphism of unitary rings, then there is just one, namely $\phi(1) = 1$ and so $\phi(m) = \phi(m \cdot 1) = m\phi(1) = m$, so just the identity.

If we allow $\phi(1) \neq 1$, then we still have that ϕ is determined by $\phi(1)$ since $\phi(m) = \phi(m \cdot 1) = m\phi(1)$. since $\phi(1 \cdot 1) = \phi(1)\phi(1) = \phi(1)$ we have $\phi(1) = k$ for some $k \in \mathbb{Z}_n$ satisfying $k^2 = k$ or $k(k - 1) = 0$. (That is $\phi(1)$ must be an idempotent element of \mathbb{Z}_n .)

We can count the number of idempotents. If $n = p_1^{m_1} \cdots p_k^{m_k}$, then

$$\mathbb{Z}_n \simeq \mathbb{Z}_{p_1^{m_1}} \times \mathbb{Z}_{p_2^{m_2}} \times \cdots \times \mathbb{Z}_{p_k^{m_k}}$$

so any idempotent k can be associated to (k_1, \dots, k_l) where each k_i is idempotent in $\mathbb{Z}_{p_i^{m_i}}$, but this means that $p_i^{m_i} \mid k_i(k_i - 1)$ and as p_i can only divide one of k_i or $k_i - 1$ we know that either $k_i = p_i^{m_i}$ or $k_i = 1$. Thus there are 2^l many idempotents and so 2^l many homomorphisms of \mathbb{Z}_n where there are l many distinct prime divisors of n .

31. Prove that $R[x]/(x^2)$ is ring isomorphic to $\left\{ \begin{bmatrix} a & b \\ 0 & a \end{bmatrix} \mid a, b \in R \right\}$.

Let $\phi(a_0 + a_1x + a_2x^2 + \cdots + a_nx^n) = \begin{bmatrix} a_0 & a_1 \\ 0 & a_0 \end{bmatrix}$. Preservation of addition is trivial. For multiplication notice

$$f(x)g(x) = (a_0 + a_1x + q(x)x^2)(b_0 + b_1x + r(x)x^2) = a_0b_0 + (a_0b_1 + a_1b_0)x + s(x)x^2$$

and so

$$\phi(f(x))\phi(g(x)) = \begin{bmatrix} a_0 & a_1 \\ 0 & a_0 \end{bmatrix} \begin{bmatrix} b_0 & b_1 \\ 0 & b_0 \end{bmatrix} = \begin{bmatrix} a_0b_0 & a_0b_1 + a_1b_0 \\ 0 & a_0b_0 \end{bmatrix} = \phi(f(x)g(x))$$

We have $f(x) \in \ker(\phi)$ iff $f(x) = 0 + 0x + q(x)x^2 \in (x^2)$, so

$$R[x]/\ker(\phi) = R[x]/(x^2) \simeq \left\{ \begin{bmatrix} a & b \\ 0 & a \end{bmatrix} \mid a, b \in R \right\}$$

34. Let $\phi : \mathbb{Z} \times \mathbb{Z} \rightarrow \mathbb{Z}_a \times \mathbb{Z}_b$ be given by $\phi(m, n) = (m \bmod a, n \bmod b)$. It is easy to see that ϕ is a surjective homomorphism.

$$(m, n) \in \ker(\phi) \iff m \bmod a = 0 \text{ and } n \bmod b = 0 \iff (m, n) \in (a) \times (b)$$

So $\mathbb{Z} \times \mathbb{Z} / \ker(\phi) = (\mathbb{Z} \times \mathbb{Z}) / ((a) \times (b)) \simeq \mathbb{Z}_a \times \mathbb{Z}_b$.

38. Let n be given in base 10 as, $n = d_k d_{k-1} \cdots d_1 d_0 = d_k 10^k + d_{k-1} 10^{k-1} + \cdots + d_1 10 + d_0$ where $d_i \in \mathbb{Z}_{10}$. Then, since $10 = -1 \bmod 11$,

$$\begin{aligned} n \bmod 11 &= d_k (10 \bmod 11)^k + d_{k-1} (10 \bmod 11)^{k-1} + \cdots + d_1 (10 \bmod 11) + d_0 \\ &= (d_k (-1)^k + d_{k-1} (-1)^{k-1} + \cdots + d_1 (-1) + d_0) \bmod 11 \end{aligned}$$

So

$$11 \mid n \iff 11 \mid d_k (-1)^k + d_{k-1} (-1)^{k-1} + \cdots + d_1 (-1) + d_0$$

40. Suppose $\phi : \mathbb{Z}_m \rightarrow \mathbb{Z}_n$ is a ring homomorphism. Then as discussed above, it must be the case that $\phi(1)$ completely determines ϕ , and it must be that $\phi(1)^2 = \phi(1)$ and $n \mid m\phi(1)$, since $\phi(0) = 0$ is required. If $\phi(1) = 1$, then we must have $n \mid m$.

44. Clearly, $R[x]/(x) \simeq R$ so (x) is maximal iff R is a field. So (x) is maximal in $\mathbb{Z}_n[x]$ iff \mathbb{Z}_n is a field iff n is prime.

46. Show that if $\phi : F \rightarrow F$ is a field homomorphism, then the prime subfield is fixed by F .

There are two ways to define the prime subfield, F_0 . The official definition is

$$F_0 = \bigcap \{F' \subseteq F \mid F' \text{ is a subfield}\}$$

Since the intersection of subfields is a subfield, this definitely defines F_0 as the minimal subfield. On the other hand, F_0 is the subfield generated by 1_F , for a field of prime characteristic p , this is just the copy of \mathbb{Z}_p generated from 1_F . For a field of characteristic 0, F_0 is the copy of \mathbb{Q} of the form $n_F m_F^{-1}$ where $m \neq 0$ and $n_F = 1_F + \cdots + 1_F$, n -times.

So, according to each definition, there is a proof. The proof using the second definition is trivial, just using the fact that $\phi(1_F) = 1_F$.

The proof using the first definition is, perhaps, more interesting. The point is that $\ker(\phi) = \{0_F\}$, assuming that $\ker(\phi) \neq F$. This is because $F/(0_F) \simeq F$ is a field, and so $(0_F) = \{0_F\}$ is a maximal ideal, so there are no non-trivial ideals, and hence every epimorphism is an automorphism. So $\phi(F_0) = \bigcap \{\phi(F') \mid F' \text{ a subfield of } F\} = \bigcap \{F' \mid F' \text{ a subfield of } F\} = F_0$. This argument would not work except that ϕ is a bijection and

$$F' \text{ is a subfield of } F \iff \phi(F') \text{ is a subfield of } \phi(F) = F$$

and

$$F' \text{ is a subfield of } \phi(F) = F \iff \phi^{-1}(F') \text{ is a subfield of } F$$

50. Prove that $x \mapsto x^p$ is a ring homomorphism in a ring of prime characteristic p . We have already done the hard work

$$\begin{aligned} (x+y)^p &= \sum_{k=0}^p \binom{p-k}{k} x^k y^{p-k} = x^p + y^p && \text{since } p \mid \binom{p-k}{k} \text{ for } 0 < k < p \\ (x \cdot y)^p &= x^p \cdot y^p && \text{trivial} \end{aligned}$$

If R is a field, then $\ker(\phi)$ can only be R or $\{0\}$. In this case $\phi(1) \neq 0$ so $\ker(\phi) = \{0\}$ and $\phi : R \rightarrow R$ is injective. Now this gets us that ϕ is an isomorphism between R and $\phi(R)$ not that $\phi \in \text{Aut}(R)$, for this we would need to assume further that every member of R has the form x^p , such a ring, or field, is called **perfect**. Any finite field is perfect, but there are imperfect infinite fields of characteristic p .

So this is an interesting problem:

Finite fields are perfect: For R finite the fact that ϕ is 1:1 implies it must be onto, and hence we actually get a proof here that every finite field is perfect.

Counter Example Let $R = \mathbb{Z}_p(t)$ be the **field** of rational functions. $t \neq f(t)^p$ for any rational function $f(t)$.

65. Let Q be the field of quotients of $\mathbb{Z}[i]$ and define $\phi : Q \rightarrow \mathbb{Q}[i]$ by $(a, b) \mapsto a \cdot b^{-1}$. We can check that this is well-defined and a field homomorphism.

To see that the map is well-defined, suppose $(a, b) = (a', b')$, that is $ab' - a'b = 0$. Then in $\mathbb{Q}[i]$ it is also true that $ab' = a'b$ and so $ab^{-1} = a'b'^{-1}$ so $\phi((a, b)) = \phi((a', b'))$.

Next we check addition, $\phi((a, b) + (a', b')) = \phi((ab' + a'b, bb')) = (ab' + a'b)(bb')^{-1} = ab^{-1} + a'b'^{-1} = \phi((a, b)) + \phi((a', b'))$. Multiplication is similar.

The map is necessarily 1-1, being a map between fields, so all that is left is seeing that it is onto. Let $r + si \in \mathbb{Q}[i]$, then $r = a/b$ and $s = a'/b'$ where $a, a', b, b' \in \mathbb{Z}$ so $r + si = (ab' + a'bi)(bb')^{-1} \in \text{Img}(\phi)$.

67. Let D be an integral domain and F the field of quotients. Let E be a field that contains D , then E contains naturally a copy of F .

This is exactly as above, define $\phi : F \rightarrow E$ by $(a, b) \mapsto ab^{-1}$. Then $\text{Img}(\phi)$ is the desired copy.